some progress based on Adam's proof framework

src/Fs9.v
@@ -2,6 +2,7 @@ Require Import List.
 Require Import Arith.
 Import ListNotations.
 Require Import CpdtTactics.
+Require Import FunctionalExtensionality.
 
 Set Implicit Arguments.
 
@@ -11,12 +12,12 @@ Definition block := nat.
 
 (* Storage *)
 
-Definition mem := addr -> value.
-Definition mem0 : mem := fun _ => 0.
-Definition st_read (m : mem) (a : addr) : value := m a.
-Definition st_write (m : mem) (a : addr) (v : value) : mem :=
-  fun a' => if eq_nat_dec a' a then v else m a'.
-Definition storage := mem.
+Definition storage := block -> value.
+Definition st_init : storage := fun _ => 0.
+Definition st_read (s:storage) (b:block) : value := s b.
+Definition st_write (s:storage) (b:block) (v:value) : storage :=
+  fun b' => if eq_nat_dec b' b then v else s b'.
+
 
 (** high-level language for a transactional disk *)
 
@@ -68,8 +69,8 @@ Fixpoint texec (p:tprog) (s:tstate) : tstate :=
   end.
 
 
-Eval simpl in texec THalt (TSt mem0 None).
-Eval simpl in texec (TWrite 0 1 (fun trs => THalt)) (TSt mem0 None).
+Eval simpl in texec THalt (TSt st_init None).
+Eval simpl in texec (TWrite 0 1 (fun trs => THalt)) (TSt st_init None).
 
 Bind Scope tprog_scope with tprog.
 
@@ -95,12 +96,12 @@ Notation "v <- a ; b" := (a (fun ra =>
 
 Open Scope tprog_scope.
 
-Eval simpl in texec THalt (TSt mem0 None).
-Eval simpl in texec (TBegin ;; THalt) (TSt mem0 None).
-Eval simpl in texec (v <- (TRead 0) ; (TWrite 0 v) ;; THalt) (TSt mem0 None).
-Eval simpl in texec (TWrite 0 1 ;; (v <- (TRead 0) ; (TWrite 1 v) ;; THalt)) (TSt mem0 None).
-Eval simpl in texec (TBegin ;; TWrite 0 1 ;; TWrite 1 1 ;; TEnd ;; THalt) (TSt mem0 None).
-Eval simpl in texec (TBegin ;; TWrite 0 1 ;; TWrite 1 1 ;; THalt) (TSt mem0 None).
+Eval simpl in texec THalt (TSt st_init None).
+Eval simpl in texec (TBegin ;; THalt) (TSt st_init None).
+Eval simpl in texec (v <- (TRead 0) ; (TWrite 0 v) ;; THalt) (TSt st_init None).
+Eval simpl in texec (TWrite 0 1 ;; (v <- (TRead 0) ; (TWrite 1 v) ;; THalt)) (TSt st_init None).
+Eval simpl in texec (TBegin ;; TWrite 0 1 ;; TWrite 1 1 ;; TEnd ;; THalt) (TSt st_init None).
+Eval simpl in texec (TBegin ;; TWrite 0 1 ;; TWrite 1 1 ;; THalt) (TSt st_init None).
 
 (* Follow adam's suggestion of "proving" this high-level language interpreter
 correct by building a simple app for which we can state the properties
@@ -115,7 +116,7 @@ Definition create_account (n : nat) (v : nat) (s: tstate): tstate :=
   texec (TBegin;; TWrite n 100 ;; TEnd ;; THalt) s.
 
 Definition transfer (src:nat) (dst:nat) (v:nat): value * value :=
-  let s := create_account src 100 (TSt mem0 None) in 
+  let s := create_account src 100 (TSt st_init None) in 
      let s1 := create_account dst 100 s in
      let s2 := do_transfer src dst v s1 in
          (read s2 src, read s2 dst).
@@ -181,7 +182,7 @@ Definition do_tbegin (cc:tprog -> pprog) rx : pprog :=
    if tx then 
     cc (rx TRFail)
    else
-    PSetTx true ;; PClrLog ;; cc (rx TRSucc)
+    PClrLog ;; PSetTx true ;; cc (rx TRSucc)
 .
 
 Definition do_tread (cc:tprog -> pprog) b rx : pprog :=
@@ -215,9 +216,9 @@ Definition do_tend (cc:tprog -> pprog) rx : pprog :=
 Definition do_trecover rx : pprog :=
   tx <- PGetTx;
   if tx then
-    PClrLog ;; rx
+    PClrLog ;; PSetTx false ;; rx
   else
-    l <- PGetLog; pflush l ;; rx
+    l <- PGetLog ; pflush l ;; PClrLog ;; rx
 .
 
 Close Scope pprog_scope.
@@ -268,9 +269,55 @@ Inductive pstep : pstate -> pprog -> pstate -> Prop :=
   | PsGetTx: forall d l c rx s,
     pstep (PSt d l c) (rx c) s ->
     pstep (PSt d l c) (PGetTx rx) s
-  | PsCrash: forall s p s',     (* we can run recovery at anytime and continue *)
+  | PsCrash: forall s p,  (* assuming the recovery process does not fail *)
+    pstep s p (pexec (do_trecover PHalt) s)
+  .
+(*| PsCrash: forall s p s',  (* we can run recovery at anytime and continue *)
     pstep s (do_trecover p) s' ->
-    pstep s p s'.
+    pstep s p s'. *)
+
+
+
+Ltac t' := simpl in *;
+  repeat (match goal with
+            | [ H : ?x = _ |- _ ] => subst x
+            | [ |- context[match ?E with pair _ _ => _ end] ] => destruct E
+            | [ |- context[if eq_nat_dec ?X ?Y then _ else _] ] => destruct (eq_nat_dec X Y)
+          end; simpl).
+Ltac t := simpl in *; intros;
+  t'; try autorewrite with core in *; intuition (eauto; try congruence); t'.
+
+Ltac step := repeat 
+  (match goal with
+   | [ H : pstep _ _ _ |- _ ] => inversion H; [|]; clear H; intros
+   end); t.
+
+(** A quick useful list lemma *)
+Theorem app_comm_cons : forall A (ls1 : list A) x ls2,
+  ls1 ++ x :: ls2 = (ls1 ++ x :: nil) ++ ls2.
+Proof.
+  induction ls1; t; rewrite IHls1; t.
+Qed.
+
+(** There's no point in two consecutive writes to the same address. *)
+Lemma upd_upd_eq : forall m a v v',
+  st_write (st_write m a v) a v' = st_write m a v'.
+Proof.
+  unfold st_write; intros; extensionality a'; t.
+Qed.
+
+Hint Rewrite upd_upd_eq.
+
+(** Writes to unequal addresses commute. *)
+Lemma upd_upd_neq : forall m a a' v v',
+  a <> a'                      
+  -> st_write (st_write m a v) a' v' = st_write (st_write m a' v') a v.
+Proof.
+  unfold st_write; intros; extensionality a''; t.
+Qed.
+
+Hint Rewrite upd_upd_eq.
+
 
 Fixpoint log_flush (p:list (block*value)) (d:storage) : storage :=
   match p with
@@ -278,17 +325,135 @@ Fixpoint log_flush (p:list (block*value)) (d:storage) : storage :=
   | (b, v) :: rest => log_flush rest (st_write d b v)
   end.
 
-Theorem correct' : forall d p l d' l' c',
-  pstep (PSt d l false) (compile_tp p) (PSt d' l' c')
-  -> d' = d \/ d' = TSDisk (texec p (TSt (log_flush l d) None)).
+(** When we're writing from the log, initial memory values don't matter in
+  * positions that will be overwritten later. *)
+Lemma writeLog_overwrite : forall a l m m' v,
+  (forall a', a' <> a -> m a' = m' a')
+  -> st_write (log_flush l m) a v = st_write (log_flush l m') a v.
 Proof.
-  induction p; intros; auto.
+  induction l; t.
+  unfold st_write; extensionality a'; t.
+  apply IHl; t.
+  unfold st_write; t.
+Qed.
+
+(** The starting value of a memory cell is irrelevant if we are writing from
+  * a log that ends in a mapping for that cell. *)
+Lemma writeLog_last : forall a v l m v',
+  log_flush (l ++ (a, v) :: nil) (st_write m a v') = st_write (log_flush l m) a v.
+Proof.
+  induction l; t.
+  destruct (eq_nat_dec a b); subst.
+  rewrite IHl.
+  apply writeLog_overwrite; unfold st_write; t.
+  rewrite upd_upd_neq by assumption; eauto.
+Qed.
+
+Hint Rewrite writeLog_last.
+
+(** Decomposing a writing process *)
+Lemma writeLog_app : forall l2 l1 m m',
+  log_flush l1 m = m'
+  -> log_flush (l1 ++ l2) m = log_flush l2 m'.
+Proof.
+  induction l1; t.
+Qed.
+
+(** [flush] implements [writeLog] in the failure-free semantics. *)
+Lemma flush_nofail : forall l m l' c,
+  pexec (pflush l (PClrLog PHalt)) (PSt m l' c) = PSt (log_flush l m) nil c.
+Proof.
+  induction l; t.
+Qed.
+
+Hint Rewrite flush_nofail app_nil_r.
+
+(** [flush] implements [writeLog] in the failure-allowed semantics. *)
+Lemma flush_writeLog' : forall l m l' m' l1 c1,
+  pstep (PSt m (l' ++ l) false) (pflush l PHalt) (PSt m' l1 c1)
+  -> log_flush l' m = m
+  -> m' = log_flush l m.
+Proof.
+  induction l; t; step.
+  rewrite app_comm_cons in *. eapply IHl. eauto. t.
+  inversion H4.
+  erewrite writeLog_app by eassumption. t.
+Qed.
+
+Lemma flush_writeLog : forall l m m' l1 c1,
+  pstep (PSt m l false) (pflush l PHalt) (PSt m' l1 c1)
+  -> m' = log_flush l m.
+Proof.
+  intros; eapply flush_writeLog' with (l':=nil) (l1:=l1) (c1:=c1); t.
+Qed.
+
+Hint Resolve flush_writeLog.
+
+(** [readLog] interacts properly with [writeLog]. *)
+Lemma readLog_correct : forall b ls d,
+  st_read (log_flush ls d) b = match pfind ls b with
+                            | Some v => v
+                            | None => st_read d b
+                          end.
+Proof.
+  induction ls; t.
+
+  destruct (pfind ls b0); eauto.
+  rewrite IHls.
+  unfold st_read, st_write; t.
+
+  destruct (pfind ls b); eauto.
+  rewrite IHls.
+  unfold st_read, st_write; t.
+Qed.
+
+(** Pulling out the effect of the last log entry *)
+Lemma writeLast_final : forall a v l m,
+  log_flush (l ++ (a, v) :: nil) m = st_write (log_flush l m) a v.
+Proof.
+  induction l; t.
+Qed.
+
+Hint Rewrite writeLast_final.
+
+Theorem correct_tx' : forall d p l d' l' c',
+  pstep (PSt d l true) (compile_tp p) (PSt d' l' c')
+  -> d' = d \/ exists ad, (TSt d' ad) = texec p (TSt d (Some (log_flush l d))).
+Proof.
+  induction p; t; step.
+
+  (* read *)
+  generalize (readLog_correct b l d).
+  destruct (pfind l b); t.
+  subst; eauto.
+  rewrite H0; inversion H11; t.
+  (* write *) eapply H in H13. t.
+  (* end *)
+  admit.
+  admit.
 Admitted.
 
-(** Main correctness theorem *)
-Theorem correct : forall d p d' l' c',
-  pstep (PSt d nil false) (compile_tp p) (PSt d' l' c')
-  -> d' = d \/ d' = TSDisk (texec p (TSt d None)).
+Theorem correct_tx : forall d p d' l' c',
+  pstep (PSt d nil true) (compile_tp p) (PSt d' l' c')
+  -> d' = d \/ exists ad, (TSt d' ad) = texec p (TSt d (Some d)).
 Proof.
-  intros. apply correct' in H. auto.
+  intros. apply correct_tx' in H . auto.
 Qed.
+
+
+Theorem correct_notx : forall d p d' l' c',
+  pstep (PSt d nil false) (compile_tp p) (PSt d' l' c')
+  -> d' = d \/ exists ad, (TSt d' ad) = texec p (TSt d None).
+Proof.
+  induction p; t; step.
+  (* XXX:
+     need to show that run a high-level program on a changed storage
+     will produce the same result as running the low-level program
+     on that storage ... *)
+  admit.
+  
+  eapply correct_tx. eassumption.
+Qed.
+
+
+(** Main correctness theorem *)
